proof/agp32_WB_CorrectScript.sml
@@ -1,4 +1,4 @@
-open hardwarePreamble translatorTheory translatorLib arithmeticTheory wordsExtraTheory dep_rewrite blastLib bitstringSyntax fcpSyntax listSyntax wordsSyntax agp32StateTheory agp32EnvironmentTheory agp32ProcessorTheory ag32Theory ag32ExtraTheory ag32UtilitiesTheory agp32RelationTheory agp32UpdateTheory agp32InternalTheory;
+open hardwarePreamble translatorTheory translatorLib arithmeticTheory wordsExtraTheory dep_rewrite blastLib bitstringSyntax fcpSyntax listSyntax wordsSyntax agp32StateTheory agp32EnvironmentTheory agp32ProcessorTheory ag32Theory ag32ExtraTheory ag32UtilitiesTheory agp32RelationTheory agp32UpdateTheory agp32InternalTheory agp32_MEM_Data_CorrectTheory;
 
 (* correctness of WB stage items with respect to the ISA *)
 val _ = new_theory "agp32_WB_Correct";
@@ -244,10 +244,136 @@ Proof
   fs [WB_pipeline_def,Rel_def,WB_Rel_def]
 QED
 
+(** WB_read_data **)
+Theorem agp32_Rel_ag32_WB_read_data_correct:
+  !fext fbits a t I.
+    is_mem fext_accessor_circuit (agp32 fext fbits) fext ==>
+    is_sch I (agp32 fext fbits) a ==>
+    Rel I (fext t) (agp32 fext fbits (t-1)) (agp32 fext fbits t) a t ==>
+    I (5,SUC t) <> NONE ==>
+    (fext (SUC t)).ready ==>
+    (agp32 fext fbits (SUC t)).WB.WB_opc = 4w ==>
+    (agp32 fext fbits (SUC t)).WB.WB_read_data = mem_data_rdata (FUNPOW Next (THE (I (5,SUC t)) − 1) a)
+Proof
+  rw [] >> Q.ABBREV_TAC `s = agp32 fext fbits t` >>
+  Q.ABBREV_TAC `s' = procs [agp32_next_state; WB_pipeline; MEM_pipeline; EX_pipeline;
+                            REG_write; ID_pipeline; IF_PC_update; Acc_compute] (fext t) s s` >>
+  Q.ABBREV_TAC `s'' = procs [IF_instr_update; ID_opc_func_update; ID_imm_update; ID_data_update;
+                             ID_data_check_update; EX_ALU_input_imm_update; EX_ALU_update;
+                             EX_SHIFT_update; EX_jump_sel_addr_update; IF_PC_input_update;
+                             MEM_ctrl_update] (fext (SUC t)) s' s'` >>
+  `(agp32 fext fbits (SUC t)).WB.WB_read_data = (WB_update (fext (SUC t)) s' s'').WB.WB_read_data`
+    by fs [agp32_WB_ctrl_items_updated_by_WB_update] >>
+  fs [WB_update_def] >>
+  IF_CASES_TAC >> fs [] >>
+  METIS_TAC [agp32_Rel_ag32_read_mem_data_rdata_correct]
+QED
+
+(** WB_read_data_byte **)
+Theorem agp32_Rel_ag32_WB_read_data_byte_correct:
+  !fext fbits a t I.
+    is_mem fext_accessor_circuit (agp32 fext fbits) fext ==>
+    is_sch I (agp32 fext fbits) a ==>
+    Rel I (fext t) (agp32 fext fbits (t-1)) (agp32 fext fbits t) a t ==>
+    I (5,SUC t) <> NONE ==>
+    (fext (SUC t)).ready ==>
+    (agp32 fext fbits (SUC t)).WB.WB_opc = 5w ==>
+    (agp32 fext fbits (SUC t)).WB.WB_read_data_byte =
+    mem_data_rdata (FUNPOW Next (THE (I (5,SUC t)) − 1) a)
+Proof
+  rw [] >> Q.ABBREV_TAC `s = agp32 fext fbits t` >>
+  Q.ABBREV_TAC `s' = procs [agp32_next_state; WB_pipeline; MEM_pipeline; EX_pipeline;
+                            REG_write; ID_pipeline; IF_PC_update; Acc_compute] (fext t) s s` >>
+  Q.ABBREV_TAC `s'' = procs [IF_instr_update; ID_opc_func_update; ID_imm_update; ID_data_update;
+                             ID_data_check_update; EX_ALU_input_imm_update; EX_ALU_update;
+                             EX_SHIFT_update; EX_jump_sel_addr_update; IF_PC_input_update;
+                             MEM_ctrl_update] (fext (SUC t)) s' s'` >>
+  `(agp32 fext fbits (SUC t)).WB.WB_read_data_byte =
+  (WB_update (fext (SUC t)) s' s'').WB.WB_read_data_byte`
+    by fs [agp32_WB_ctrl_items_updated_by_WB_update] >>
+  `s''.WB.WB_dataA = (agp32 fext fbits (SUC t)).WB.WB_dataA`
+    by METIS_TAC [agp32_same_WB_items_before_WB_update,Abbr `s`,Abbr `s'`,Abbr `s''`] >>
+  `(agp32 fext fbits (SUC t)).WB.WB_dataA = dataA (FUNPOW Next (THE (I' (5,SUC t)) − 1) a)`
+    by gs [is_sch_def,agp32_Rel_ag32_WB_dataA_correct] >>
+  fs [WB_update_def] >>
+  IF_CASES_TAC >> fs [MUX_41_def] >>
+  `opc (FUNPOW Next (THE (I' (5,SUC t)) − 1) a) = 5w`
+    by METIS_TAC [is_sch_def,agp32_Rel_ag32_WB_opc_correct] >>
+  `(fext (SUC t)).data_rdata = mem_data_rdata_extra (FUNPOW Next (THE (I' (5,SUC t)) − 1) a)`
+    by METIS_TAC [agp32_Rel_ag32_read_mem_byte_data_rdata_correct] >>
+  rw [mem_data_rdata_def,mem_data_rdata_extra_def,mem_data_addr_def] >>
+  qpat_abbrev_tac `a1 = FUNPOW Next _ a` >>
+  fs [word_at_addr_def,align_addr_def,addr_add] >>
+  Cases_on_word_value `(1 >< 0) (dataA a1)` >>
+  `dataA a1 = (31 >< 2) (dataA a1) @@ (1 >< 0) (dataA a1)` by rw [addr_split] >> gs [] >>
+  FULL_SIMP_TAC (std_ss++WORD_ss++WORD_EXTRACT_ss) [] >> METIS_TAC []                       
+QED
+
+(** WB_isOut **)
+Theorem agp32_Rel_ag32_WB_isOut_correct:
+  !fext fbits a t I.
+    is_sch_writeback I (agp32 fext fbits) ==>
+    is_sch_disable I (agp32 fext fbits) ==>
+    Rel I (fext t) (agp32 fext fbits (t-1)) (agp32 fext fbits t) a t ==>
+    I (5,SUC t) <> NONE ==>
+    ((agp32 fext fbits (SUC t)).WB.WB_isOut <=> isOut_isa (FUNPOW Next (THE (I (5,SUC t)) − 1) a))
+Proof
+  rw [] >> Q.ABBREV_TAC `s = agp32 fext fbits t` >>
+  Q.ABBREV_TAC `s' = procs [agp32_next_state; WB_pipeline; MEM_pipeline; EX_pipeline;
+                            REG_write; ID_pipeline; IF_PC_update; Acc_compute] (fext t) s s` >>
+  Q.ABBREV_TAC `s'' = procs [IF_instr_update; ID_opc_func_update; ID_imm_update; ID_data_update;
+                             ID_data_check_update; EX_ALU_input_imm_update; EX_ALU_update;
+                             EX_SHIFT_update; EX_jump_sel_addr_update; IF_PC_input_update;
+                             MEM_ctrl_update] (fext (SUC t)) s' s'` >>
+  `(agp32 fext fbits (SUC t)).WB.WB_isOut = (WB_update (fext (SUC t)) s' s'').WB.WB_isOut`
+    by fs [agp32_WB_ctrl_items_updated_by_WB_update] >>
+  `s''.WB.WB_opc = (agp32 fext fbits (SUC t)).WB.WB_opc`
+    by METIS_TAC [agp32_same_WB_items_before_WB_update,Abbr `s`,Abbr `s'`,Abbr `s''`] >>
+  `(s''.WB.WB_state_flag = (agp32 fext fbits t).WB.WB_state_flag) /\
+  (s''.WB.WB_isOut = s.WB.WB_isOut)`
+    by METIS_TAC [agp32_same_WB_items_until_WB_update,Abbr `s`,Abbr `s'`,Abbr `s''`] >>
+  fs [WB_update_def] >>
+  IF_CASES_TAC >> fs [] >-
+   (rw [isOut_isa_def] >> METIS_TAC [agp32_Rel_ag32_WB_opc_correct]) >>
+  `I' (5,SUC t) = I' (5,t)` by fs [is_sch_disable_def,enable_stg_def] >>
+  fs [Rel_def,WB_Rel_def]
+QED
+
+(** WB_data_sel **)
+Theorem agp32_Rel_ag32_WB_data_sel_correct:
+  !fext fbits a t I.
+    is_sch_writeback I (agp32 fext fbits) ==>
+    is_sch_disable I (agp32 fext fbits) ==>
+    Rel I (fext t) (agp32 fext fbits (t-1)) (agp32 fext fbits t) a t ==>
+    I (5,SUC t) <> NONE ==>
+    (agp32 fext fbits (SUC t)).WB.WB_data_sel = reg_wdata_sel (FUNPOW Next (THE (I (5,SUC t)) − 1) a)
+Proof
+  rw [] >> Q.ABBREV_TAC `s = agp32 fext fbits t` >>
+  Q.ABBREV_TAC `s' = procs [agp32_next_state; WB_pipeline; MEM_pipeline; EX_pipeline;
+                            REG_write; ID_pipeline; IF_PC_update; Acc_compute] (fext t) s s` >>
+  Q.ABBREV_TAC `s'' = procs [IF_instr_update; ID_opc_func_update; ID_imm_update; ID_data_update;
+                             ID_data_check_update; EX_ALU_input_imm_update; EX_ALU_update;
+                             EX_SHIFT_update; EX_jump_sel_addr_update; IF_PC_input_update;
+                             MEM_ctrl_update] (fext (SUC t)) s' s'` >>
+  `(agp32 fext fbits (SUC t)).WB.WB_data_sel = (WB_update (fext (SUC t)) s' s'').WB.WB_data_sel`
+    by fs [agp32_WB_ctrl_items_updated_by_WB_update] >>
+  `s''.WB.WB_opc = (agp32 fext fbits (SUC t)).WB.WB_opc`
+    by METIS_TAC [agp32_same_WB_items_before_WB_update,Abbr `s`,Abbr `s'`,Abbr `s''`] >>
+  `(s''.WB.WB_state_flag = (agp32 fext fbits t).WB.WB_state_flag) /\
+  (s''.WB.WB_data_sel = s.WB.WB_data_sel)`
+    by METIS_TAC [agp32_same_WB_items_until_WB_update,Abbr `s`,Abbr `s'`,Abbr `s''`] >>
+  fs [WB_update_def] >>
+  IF_CASES_TAC >> fs [] >-
+   (simp [reg_wdata_sel_def] >> METIS_TAC [agp32_Rel_ag32_WB_opc_correct]) >>
+  `I' (5,SUC t) = I' (5,t)` by fs [is_sch_disable_def,enable_stg_def] >>
+  fs [Rel_def,WB_Rel_def]
+QED
+
 
 (* WB_Rel *)
 Theorem agp32_Rel_ag32_WB_Rel_correct:
   !fext fbits a t I.
+    is_mem fext_accessor_circuit (agp32 fext fbits) fext ==>
     is_sch I (agp32 fext fbits) a ==>
     Rel I (fext t) (agp32 fext fbits (t-1)) (agp32 fext fbits t) a t ==>
     I (5,SUC t) <> NONE ==>
@@ -257,7 +383,9 @@ Proof
   fs [agp32_Rel_ag32_WB_PC_correct,agp32_Rel_ag32_WB_addrW_correct,agp32_Rel_ag32_WB_opc_correct,
       agp32_Rel_ag32_WB_dataA_correct,agp32_Rel_ag32_WB_imm_correct_not_LoadUpperConstant,
       agp32_Rel_ag32_WB_imm_correct_LoadUpperConstant,agp32_Rel_ag32_WB_ALU_res_correct,
-      agp32_Rel_ag32_WB_SHIFT_res_correct,agp32_Rel_ag32_WB_write_reg_correct] >>
+      agp32_Rel_ag32_WB_SHIFT_res_correct,agp32_Rel_ag32_WB_write_reg_correct,
+      is_sch_def,agp32_Rel_ag32_WB_read_data_correct,agp32_Rel_ag32_WB_read_data_byte_correct,
+      agp32_Rel_ag32_WB_isOut_correct,agp32_Rel_ag32_WB_data_sel_correct] >>
   cheat
 QED
 
